\section{Problem 1}
the exercise is to compute the partial derivations of the following
three problems each containing a different function.
\subsection{(a)}
Considering the function, it is fairly straight forward to compute the derivative with respect
to x and y. Both derivations will be done using the power rule: $x^n = nx^{n-1}$
$$f(x,y) = x^4y^3+x^5-e^y$$
\textbf{Answer:}
\\
calculating $\frac{\partial}{\partial x}$
$$f'_{x} = 4x^3y^3+5x^4$$
calculating $\frac{\partial}{\partial y}$
$$f'_{y} = x^43y^2-e^y$$
It is worth mentioning, that the exponent ($e^y$) will derive to itself even though
the power function states otherwise.
\subsection{(b)}
This function is bit harder to compute. I will be using the power rule: $x^n = nx^{n-1}$ and the chain rule: $f(g(x)) = f'(g(x)) \cdot g'(x)$
$$f(x,y) = \frac{1}{\sqrt{x^3+xy+y^2}}$$
I will start by deriving the innter function with respect to x and y since these derivations
are going to be used later on in the calculations.
\\
\\
calculating $\frac{\partial}{\partial x}$
$$f'_{x} = 3x^2+y$$
calculating $\frac{\partial}{\partial y}$
$$f'_{y} = x+2y$$
\textbf{Answer:}\\
I will rewrite the function using simple fraction rules in order to make the function
a bit easier to work with.
$$f(x,y) = (x^3+xy+y^2)^{-\frac{1}{2}}$$
applying the power rule
$$f(x,y) = -\frac{1}{2}(x^3+xy+y^2)^{-\frac{3}{2}}$$
applying the chain rule
$$f(x,y) = -\frac{1}{2}(x^3+xy+y^2)^{-\frac{3}{2}} \cdot (3x^2+y)$$
calculating $\frac{\partial}{\partial x}$
$$f'_{x} = -\frac{3x^2+y}{2(x^3+xy+y^2)^{\frac{3}{2}}}$$
I will not be showing the full calculation for $f'_{y}$ since it derives trivially in the same was as $f'_{x}$,
with the only exception being that instead of using the chain rule with the derivation of x you now use the derivative of y
thus I will only show the last two steps
\\
\\
applying the chain rule
$$f(x,y) = -\frac{1}{2}(x^3+xy+y^2)^{-\frac{3}{2}} \cdot (x^43y^2-e^y)$$
calculating $\frac{\partial}{\partial x}$
$$f'_{x} = -\frac{x+2y}{2(x^3+xy+y^2)^{\frac{3}{2}}}$$
\subsection{(c)}
I order to compute this function I will be using the power rule: $x^n = nx^{n-1}$ and the quotient rule: $(\frac{f(x)}{g(x)})' = \frac{g(x)f'(x) - f(x)g'(x)}{g(x)^2}$
$$f(x,y) = \frac{x^3+y^2}{x+y}$$
\textbf{Answer:}\\
I will start by finding the derivations for f(x) and f(y) aswell for g(x) and g(y). these calulations are done using the power rule. 
Having these calculating done, it's a simple matter of substituting with the "new" expressions in the qoutient rule
\\
$f'_{x} \cdot g(x) = 3x^2(x+y)$\\
$f'_{y} \cdot g(y) = 2y(x+y)$\\
$f(x) \cdot g'_{x} = 1\cdot(x^3+y^2)$\\
$f(y) \cdot g'_{y} = 1\cdot(x^3+y^2)$\\
\\
\\
$$f'_{x} = \frac{3x^2(x+y) - (x^3+y^2)}{(x+y)^2}$$
$$f'_{y} = \frac{2y(x+y)) - (x^3+y^2)}{(x+y)^2}$$