\section{Problem 1}
\subsection{(a)}
$$ \mathcal{L} = \frac{1}{N} \sum\limits_{n=1}^{N} \alpha_{n} (\mathbf{w}^{T} \mathbf{x}_{n} - t_{n})^2 $$ 

$$  = \frac{1}{N} (\textbf{Xw}-t)^{T} A(\textbf{Xw}-t) $$

$$  = \frac{1}{N} (\textbf{Xw})^{T} - t^{T} (A\textbf{Xw}-At) $$

$$ \frac{1}{N} (\textbf{Xw})^{T} A\textbf{Xw} - \frac{1}{N} (\textbf{Xw})^{T} At  - \frac{1}{N} A\textbf{Xw}t^{T} + \frac{1}{N} Att^{T} $$

$$  = \frac{1}{N} \textbf{w}^{T} \textbf{X}^{T} A \textbf{Xw} - \frac{2}{N}\textbf{w}^{T}\textbf{X}^T A t + \frac{1}{N}t^{T} A t $$
\\
using case 4 and case 1 from the table 1.14 when differentiating I get:
\\
$$\frac{\partial\mathcal{L}}{\partial w} = 2 \textbf{X}^{T} \textbf{A} \textbf{Xw} - 2 \textbf{X}^{T} \textbf{A} t = 0$$
\\
\\
+2 and -2 cancel out leaving me with 
$$ \textbf{X}^{T} \textbf{A} \textbf{Xw} - \textbf{X}^{T} \textbf{A} t = 0 $$
$$ \textbf{X}^{T} \textbf{A} \textbf{Xw} = \textbf{X}^{T} \textbf{A} t $$
\\
multiplying both sides with the identity matrix
\\
$$ \textbf{I}\textbf{w} = (\textbf{X}^{T} \textbf{A} \textbf{X})^{-1} \textbf{X}^{T} \textbf{A} t $$
\\
Multiplying the vector \textbf{w} with the Identity matrix, will simply return the vector \textbf{w} thus the result is
$$ \hat{\textbf{w}} = (\textbf{X}^{T} \textbf{A} \textbf{X})^{-1} \textbf{X}^{T} \textbf{A} t $$
